Examples/EdmondsKarp_Maxflow/EdmondsKarp_Time.thy
@@ -1,0 +1,61 @@
+theory EdmondsKarp_Time
+imports EdmondsKarp_Impl "SepLogicTime_RBTreeBasic.Asymptotics_2D"
+begin
+ 
+
+definition cost' :: "nat \<times> nat \<Rightarrow> nat" 
+  where "cost' = (\<lambda>(cV,cE). 
+    (
+      3 + rbt_insert_logN 1 + rbt_insert_logN 1 + 10
+       +
+         (1 + cV + cV * cV)   
+         *
+          (
+            10 + 10 + rbt_delete_time_logN (cV + 1) + 10 + 10 + (2 + cV * (1 + 1))
+             + 
+                  cV
+                   *
+                  (rbt_search_time_logN (1 + cV) + 1 + max (rbt_insert_logN (cV + 1) + rbt_insert_logN (1 + cV)) 1)
+          )
+       +
+          cV * (rbt_search_time_logN (1 + cV) + 1 + 1)
+       +
+          (1 + (1 + 10) * cV + (1 + cV * (2 * 1 + 2 * 1 + 3)))
+    )  
+   *
+    (2 * cV * cE + cV + 1)        (* O(V*E) - fofu iterations *)
+  )"
+
+fun f_sum :: "nat \<times> nat \<Rightarrow> nat" where
+  "f_sum (n,m) = n + m"
+
+lemma f_sum_asym [asym_bound]: "f_sum \<in> \<Theta>\<^sub>2(\<lambda>x. real (fst x) + real (snd x))"
+  apply (subst surjective_pairing) unfolding f_sum.simps by auto2
+
+fun cost2 :: "nat \<times> nat \<Rightarrow> nat" where "cost2 (cV,cE) = (3 + 1 + 1 + 10 +
+     (1 + cV + cV * cV) )"
+
+lemma "cost2 \<in> \<Theta>\<^sub>2(\<lambda>(V,E). real V * real V)"
+  apply (subst surjective_pairing) unfolding cost2.simps by auto2
+ 
+fun cost3 :: "nat \<times> nat \<Rightarrow> nat" where "cost3 (cV,cE) = rbt_search_time_logN ( cV)"
+
+thm rbt_search_time_logN_bound
+lemma "cost3 \<in> \<Theta>\<^sub>2(\<lambda>(V::nat,E::nat). ln V)"
+  apply (subst surjective_pairing) unfolding cost3.simps by auto2 (* ? ? ? *)
+
+lemma rbt_search_time_logN_bound[asym_bound]:
+  "(\<lambda>n. rbt_search_time_logN n) \<in> \<Theta>(\<lambda>n. ln n)" unfolding rbt_search_time_logN_def rbt_search_time_def by auto2
+
+lemma "cost3 \<in> \<Theta>\<^sub>2(\<lambda>(V::nat,E::nat). ln V)"
+  apply (subst surjective_pairing) unfolding cost3.simps by auto2
+
+
+definition edka_cost' :: "nat \<times> nat \<Rightarrow> nat" 
+    where "edka_cost' = (\<lambda>(cV,cE). 3 + rbt_insert_logN cV + rbt_insert_logN cV + 10)"
+
+lemma "edka_cost' \<in> \<Theta>\<^sub>2(\<lambda>(V,E). ln V)"
+  apply (subst surjective_pairing) unfolding edka_cost_def by auto2
+ 
+
+end
